\documentclass{article}

\usepackage[utf8]{inputenc}
\usepackage[english]{babel}
\usepackage[foundations]{../lib/tex/naproche}


\title{Sum of an Arithmetic Series}
\author{}
\date{}

\begin{document}
\maketitle

\begin{forthel}
    [prove off][check off]

    [readtex \path{100_Theorems.ftl.tex}]

    [prove on][check on]
  \end{forthel}

\section{* Sum of an Arithmetic Series}

\newcommand{\sumarith}[3]{\sum_{i = 1}^{#3}(#1 + #2 \cdot i)}

\begin{forthel}
Let $a,d$ denote real numbers.
Let $n$ denote a natural number.

\begin{signature}
$\sumarith{a}{d}{n}$ is a real number.
\end{signature}

\begin{axiom}
$\sumarith{a}{d}{1} = a + d$.
\end{axiom}

\begin{axiom}[1]
$\sumarith{a}{d}{n+1} = \sumarith{a}{d}{n} + (a + (d \cdot (n + 1)))$.
\end{axiom}

[timelimit 5]
\begin{theorem} For all nonzero natural numbers $n$
$$\sumarith{a}{d}{n} = n \cdot ( a + \frac{(n + 1) \cdot d}{2}).$$
\end{theorem}
\begin{proof}[by induction on $n$]
Let $n$ be a nonzero natural number.

Case $n = 1$.
Trivial.

Take a natural number $m$ such that $m + 1 = n$. $m$ is inductively smaller than $n$.

$$\sumarith{a}{d}{m} = m \cdot ( a + \frac{(m + 1) \cdot d}{2}).$$

Then
$$\sumarith{a}{d}{n} = 
(m \cdot ( a + \frac{(m + 1) \cdot d}{2})) + (a + (d \cdot (m + 1)))$$
(by 1).


Hence

$\sumarith{a}{d}{n} =$

$((m \cdot a) + (m \cdot \frac{n \cdot d}{2})) + (a + (d \cdot n)) =$

$(((m \cdot a) + a) +  (m \cdot \frac{n \cdot d}{2})) + (d \cdot n) =$

$(((m \cdot a) + (1 \cdot a)) +  (m \cdot \frac{n \cdot d}{2})) + (d \cdot n) =$

$((n \cdot a) +  (m \cdot \frac{n \cdot d}{2})) + (d \cdot n)$.

$((n \cdot a) +  (m \cdot \frac{n \cdot d}{2})) + (d \cdot n) =$

$(n \cdot a) +  ((m \cdot \frac{n \cdot d}{2}) + (d \cdot n))=$

$(n \cdot a) +  ((m \cdot \frac{n \cdot d}{2}) + (1 \cdot (d \cdot n)))=$

$(n \cdot a) +  ((m \cdot \frac{n \cdot d}{2}) + (\frac{2}{2} \cdot (d \cdot n)))$.

Then $(n \cdot a) +  ((m \cdot \frac{n \cdot d}{2}) + (\frac{2}{2} \cdot (d \cdot n))) =$

$(n \cdot a) +  ((m \cdot \frac{n \cdot d}{2}) + (2 \cdot \frac{n \cdot d}{2})) =$

$(n \cdot a) +  ((m +2) \cdot \frac{n \cdot d}{2})$.

Then $(n \cdot a) +  ((m +2) \cdot \frac{n \cdot d}{2}) =$

$(n \cdot a) +  ((n+1) \cdot \frac{n \cdot d}{2}) =$

$(n \cdot a) +  \frac{(n+1) \cdot (n \cdot d)}{2} =$

$(n \cdot a) +  \frac{n \cdot ((n+1) \cdot d)}{2} =$

$(n \cdot a) +  (n \cdot \frac{((n+1) \cdot d)}{2}) =$

$n \cdot ( a + \frac{(n + 1) \cdot d}{2})$.
\end{proof}
\end{forthel}

\end{document}
