\documentclass{article}

\usepackage[utf8]{inputenc}
\usepackage[english]{babel}
\usepackage[foundations]{../lib/tex/naproche}


\title{Irrationality of the Square Root of 2}
\author{}
\date{}



\begin{document}
\maketitle

\begin{forthel}
    [prove off][check off]

    [readtex \path{100_Theorems.ftl.tex}]
    [readtex \path{W-bezout.ftl.tex}]

    [prove on][check on]
  \end{forthel}

\section{* The Irrationality of the Square Root of 2}



\begin{forthel}

Let a prime number stand for a prime natural number.
Let $p$ denote a prime number.


\begin{definition}
    Let $n,m$ be integers.
    $n$ and $m$ are coprime iff $n$ and $m$ have no common divisor $d$ such that $d$ is a prime number.
\end{definition}

\begin{lemma}
    For all rational numbers $q$ there exist coprime integers $m,n$ such that $m \cdot q = n$.
\end{lemma}



Let $n$ denote an integer.
\begin{lemma}
    If $p$ divides $n^{2}$ then $p$ divides $n$.
\end{lemma}
%\begin{proof}
%    Assume $p$ divides $n^{2}$ and $p$ not divides $n$. $p$ not divides $n$ and $\gcd(p,n)=1$.
%    There exist integers $j,k$ such that $(k \cdot n) + (j \cdot p) = 1$.
%    Let $k,j$ be integers such that $(k \cdot n) + (j \cdot p) = 1$.
%    $n^{2} = n \cdot n^{1} = n \cdot n$.
%    $p$ divides $k \cdot (n \cdot n)$ and $p$ divides $(j \cdot p) \cdot n$.
%    Then $p$ divides $(k \cdot (n \cdot n)) + ((j \cdot p) \cdot n)$.
%    $(k \cdot n^{2}) + ((j \cdot p) \cdot n) = (k \cdot (n \cdot n)) + ((j \cdot p) \cdot n)$.
%    Then $((k \cdot n) \cdot n) + ((j \cdot p) \cdot n) = ((k \cdot n) + (j \cdot p)) \cdot n = 1 \cdot n = n$.
%    Thus $p$ divides $n$. 
%\end{proof}



\begin{proposition}
    $q^{2} = p$ for no rational number $q$.
\end{proposition}
%\begin{proof}[by contradiction]
%    Assume the contrary.
%    Take a positive rational number $q$ such that $p = q^{2}$.
%    Take coprime natural numbers $m,n$ such that $m \cdot q = n$.
%    Then $(m \cdot q) \cdot n = n^{2}$. 
%    Then  $(m \cdot q) \cdot n = (m \cdot q) \cdot (m \cdot q) = ((m \cdot q) \cdot m) \cdot q$.
%    $((m \cdot q) \cdot m) \cdot q  = (m^{2} \cdot q) \cdot q = m^{2} \cdot q^{2}$.
%    $m^{2} \cdot q^{2} = n^{2}.$
%    Then $p \cdot m^{2} = n^{2}$.
%    $p$ divides $n^{2}$. Therefore $p$ divides $n$.
%    Take a natural number $k$ such that $n = k \cdot p$.
%    Then $p \cdot m^{2} = p \cdot (k \cdot n)$.
%    Therefore $m \cdot m$ is equal to $p \cdot k^{2}$.
%    Hence $p$ divides $m$.
%    Contradiction.
%\end{proof}
\end{forthel}

\end{document}