\documentclass{article}
\usepackage[english]{babel}
\usepackage{../lib/tex/naproche}

\begin{document}    

\section{Sum of a Geometric Series (Wiedijk \# 66)}

\newcommand{\sumgeom}[2]{\sum_{0 \leq i < #2} {#1}^i}

In this document we give a proof of the Sum of a Geometric Series:

\begin{forthel}
[prove off]
[readtex \path{100_Theorems.ftl.tex}]
[prove on]


Let $x$ denote real number. 


\begin{theorem} Let $x \neq 1$. Then
$$\sumgeom{x}{n} = \frac{1 - x^{n}}{1 - x}$$
for all natural numbers $n$.
\end{theorem}
\begin{proof}[by induction on $n$]

$1 - x \neq 0$.

Let $n$ be a natural number.

Case $n = 0$. Trivial.

Take a natural number $m$ such that $m + 1 = n$. 
$m$ is inductively smaller than $m+1$ and
$\sumgeom{x}{m} = \frac{1 - x^{m}}{1 - x}$.


Let $a = x^{m}$ and $b = x^{n}$ and $c=1-x$.
Then $a,b,c$ are real numbers and
$\sumgeom{x}{n} =
\frac{1 - x^{m}}{1 - x} + x^{m} = 
\frac{1 - x^{m}}{1 - x} + \frac{x^{m} \cdot (1-x)}{1 - x} =
\frac{1 - x^{m}}{1 - x} + \frac{(x^{m} \cdot 1) + (x^{m} \cdot (-x))}{1 - x} = 
\frac{1 - x^{m}}{1 - x} + \frac{x^{m} + ((-x) \cdot x^{m})}{1 - x} =
\frac{1 - x^{m}}{1 - x} + \frac{x^{m} + (-(x \cdot x^{m}))}{1 - x} =
\frac{1 - x^{m}}{1 - x} + \frac{x^{m} - x^{n}}{1 - x} = 
\frac{1 - a}{c} + \frac{a - b}{c} =
\frac{1 - b}{c} = 
\frac{1 - x^{n}}{1 - x}$.

\end{proof}

\end{forthel}